half way through unification

typeclass/typing/typeclass_unificationScript.sml
@@ -10,26 +10,17 @@ open typeclass_typesTheory typeclass_inference_commonTheory;
 
 val _ = new_theory "typeclass_unification";
 
-(*
-Datatype:
-  utype = uDBVar num
-        | uPrimTy prim_ty
-        | uException
-        | uTypeCons (num + comp_prim_ty)
-End
-*)
-
 Definition encode_itype_def[nocompute]:
-  encode_itype (Atom at) = Const at
-  encode_itype (CVar n) = Var n
-  encode_itype (Cons it1 it2) = Pair (encode_itype it1) (encode_itype it2)
+  encode_itype (iAtom at) = Const at ∧
+  encode_itype (iCVar n) = Var n ∧
+  encode_itype (iCons it1 it2) = Pair (encode_itype it1) (encode_itype it2)
 End
 
-Definition decode_utype_acc_def[nocompute]:
+Definition decode_utype_def[nocompute]:
   decode_utype (Pair u1 u2) =
-    Cons (decode_utype u1) (decode_utype u2) ∧
-  decode_utype_acc (Const $ at) = Atom at ∧
-  decode_utype_acc (Var n) = CVarCons n ∧
+    iCons (decode_utype u1) (decode_utype u2) ∧
+  decode_utype (Const $ at) = iAtom at ∧
+  decode_utype (Var n) = iCVar n
 End
 
 Triviality I_o_f:
@@ -53,13 +44,13 @@ QED
 Theorem decode_encode:
   ∀it. decode_utype (encode_itype it) = it
 Proof
-  simp[decode_utype_def,AND_CLAUSES,CONJ_ASSOC] >>
-  Induct >>
-  rw[encode_itype_def, decode_utype_acc_def]
+  Induct >> rw[encode_itype_def, decode_utype_def]
 QED
 
 Theorem encode_decode:
+  ∀ut. encode_itype (decode_utype ut) = ut
 Proof
+  Induct >> rw[encode_itype_def,decode_utype_def]
 QED
 
 Definition pure_wfs_def[nocompute]:
@@ -67,12 +58,12 @@ Definition pure_wfs_def[nocompute]:
 End
 
 Definition pure_vwalk_def[nocompute]:
-  pure_vwalk s v = THE $ decode_utype (vwalk (encode_itype o_f s) v)
+  pure_vwalk s v = decode_utype (vwalk (encode_itype o_f s) v)
 End
 
 Theorem pure_vwalk_ind:
   ∀s. pure_wfs s ⇒
-    ∀P. (∀v. (∀w u. FLOOKUP s v = SOME (CVarCons u []) ⇒ P u) ⇒ P v) ⇒ ∀v. P v
+    ∀P. (∀v. (∀w u. FLOOKUP s v = SOME (iCVar u) ⇒ P u) ⇒ P v) ⇒ ∀v. P v
 Proof
   ntac 4 strip_tac >> gvs[pure_wfs_def] >>
   drule $ DISCH_ALL vwalk_ind >> disch_then irule >> rw[] >>
@@ -86,36 +77,31 @@ Theorem pure_vwalk:
     ∀v.
       pure_vwalk s v =
         case FLOOKUP s v of
-        | NONE => CVarCons v []
-        | SOME (CVarCons w []) => pure_vwalk s w
+        | NONE => iCVar v
+        | SOME (iCVar w) => pure_vwalk s w
         | SOME t => t
 Proof
   rw[pure_vwalk_def, pure_wfs_def] >>
   CASE_TAC >> gvs[] >>
   simp[Once vwalk_def, FLOOKUP_o_f,
-    decode_utype_def, decode_utype_acc_def] >>
-  Cases_on `x` using itype_SNOC_CASES >>
-  gvs[encode_itype_alt,decode_encode,decode_utype_acc_def] >>
-  simp[list_case_eq] >>
-  metis_tac[list_nchotomy,APPEND_eq_NIL]
+    decode_utype_def] >>
+  Cases_on `x` >>
+  simp[encode_itype_def,decode_utype_def,decode_encode]
 QED
 
 Definition pure_walk_def[nocompute]:
-  pure_walk s t = THE $ decode_utype (walk (encode_itype o_f s) (encode_itype t))
+  pure_walk s t = decode_utype (walk (encode_itype o_f s) (encode_itype t))
 End
 
 Theorem pure_walk:
   ∀s t. pure_walk s t =
     case t of
-    | CVarCons v [] => pure_vwalk s v
+    | iCVar v => pure_vwalk s v
     | t => t
 Proof
   rw[pure_walk_def, pure_vwalk_def, walk_def] >>
-  Cases_on `t` using itype_SNOC_CASES >>
-  simp[encode_itype_alt] >>
-  gvs[decode_utype_def,decode_utype_acc_def,decode_encode] >>
-  simp[list_case_eq] >>
-  metis_tac[list_nchotomy,APPEND_eq_NIL]
+  Cases_on `t` >>
+  simp[encode_itype_def,decode_utype_def,decode_encode]
 QED
 
 Definition pure_oc_def[nocompute]:
@@ -126,14 +112,6 @@ Definition pure_vars_def[nocompute]:
   pure_vars t = vars (encode_itype t)
 End
 
-Triviality SNOC_CONS:
-  ∀t ts. ?h l. SNOC t ts = CONS h l
-Proof
-  metis_tac[list_nchotomy,rich_listTheory.NOT_SNOC_NIL]
-QED
-
-Triviality EXISTS_
-
 Theorem encode_vwalk:
   ∀s. pure_wfs s ⇒
     ∀u. vwalk (encode_itype o_f s) u = encode_itype (pure_vwalk s u)
@@ -143,12 +121,8 @@ Proof
   `wfs (encode_itype o_f s)` by metis_tac [pure_wfs_def] >>
   rw [Once vwalk_def, Once pure_vwalk, FLOOKUP_o_f] >>
   Cases_on `FLOOKUP s v` >> rw [encode_itype_def] >>
-  Cases_on `x` using itype_SNOC_CASES >>
-  gvs[encode_itype_alt] >>
-  qspecl_then [`t`,`ts`] strip_assume_tac SNOC_CONS >>
-  simp[] >>
-  pop_assum $ assume_tac o GSYM >>
-  simp[encode_itype_alt]
+  Cases_on `x` >>
+  simp[encode_itype_def]
 QED
 
 Theorem pure_oc_lemma:
@@ -165,31 +139,23 @@ Theorem pure_oc:
     ∀t v.
       pure_oc s t v =
         case pure_walk s t of
-        | CVarCons u [] => v = u
-        | CVarCons u its => (pure_oc s (CVarCons u []) v) ∨
-            EXISTS (λit. pure_oc s it v) its
-        | TypeCons n its => EXISTS (λit. pure_oc s it v) its
-        | DBVarCons n its => EXISTS (λit. pure_oc s it v) its
-        | _ => F
+        | iCVar u => v = u
+        | iCons l r => pure_oc s l v ∨ pure_oc s r v
+        | iAtom a => F
 Proof
   rw[pure_oc_def] >>
   `wfs (encode_itype o_f s)` by fs [pure_wfs_def] >>
   rw[Once oc_walking, pure_walk_def, walk_def] >>
-  Cases_on `t` using itype_SNOC_CASES >>
-  simp[encode_itype_alt, decode_utype_def,
-    decode_utype_acc_def, decode_encode,
-    encode_vwalk, pure_oc_lemma] >>
-  Cases_on `pure_vwalk s n` using itype_SNOC_CASES >>
-  rw[encode_itype_alt, pure_oc_lemma, EXISTS_SNOC, DISJ_COMM,
-    encode_vwalk] >>
-  Cases_on `ts` >>
-  simp[EXISTS_SNOC] >>
-  metis_tac[]
+  Cases_on `t` >>
+  simp[encode_itype_def,decode_utype_def,
+    decode_encode,encode_vwalk] >>
+  Cases_on `pure_vwalk s n` >>
+  simp[encode_itype_def,encode_vwalk]
 QED
 
 Definition pure_ext_s_check_def[nocompute]:
   pure_ext_s_check s v t =
-    OPTION_MAP ((o_f) (THE o decode_utype)) $
+    OPTION_MAP ($o_f decode_utype) $
       ext_s_check (encode_itype o_f s) v (encode_itype t)
 End
 
@@ -203,20 +169,9 @@ QED
 
 Definition pure_unify_def[nocompute]:
   pure_unify s t1 t2 =
-    OPTION_MAP ((o_f) (THE o decode_utype)) $
+    OPTION_MAP ($o_f decode_utype) $
       unify (encode_itype o_f s) (encode_itype t1) (encode_itype t2)
 End
-
-(*
-Definition pure_unifyl_def:
-  pure_unifyl s [] [] = SOME s ∧
-  pure_unifyl s (t1::ts1) (t2::ts2) = (
-    case pure_unify s t1 t2 of
-    | NONE => NONE
-    | SOME s' => pure_unifyl s' ts1 ts2) ∧
-  pure_unifyl s _ _ = NONE
-End
-*)
 
 Theorem encode_walk:
   ∀s. pure_wfs s ⇒
@@ -231,21 +186,18 @@ QED
 
 Theorem encode_pair_cases:
   ∀t t1 t2. encode_itype t = Pair t1 t2 ⇒
-    (∃c ts. t1 = Const (uTypeCons c) ∧ t2 = encode_itypes ts) ∨
-    (∃ts. t1 = Const uTuple ∧ t2 = encode_itypes ts) ∨
-    (∃it1 it2. t1 = Const uFunction ∧
-               t2 = Pair (encode_itype it1) (encode_itype it2)) ∨
-    (∃t. t1 = Const uArray ∧ t2 = encode_itype t) ∨
-    (∃t. t1 = Const uM ∧ t2 = encode_itype t)
+    ∃t1' t2'.
+      t1 = (encode_itype t1') ∧
+      t2 = (encode_itype t2') ∧
+      t = iCons t1' t2'
 Proof
-  Cases >> rw[encode_itype_def] >> rpt $ irule_at Any EQ_REFL
+  Cases >> rw[encode_itype_def]
 QED
 
 Theorem encode_itype_injective:
-  (∀t1 t2. encode_itype t1 = encode_itype t2 ⇔ t1 = t2) ∧
-  (∀t1s t2s. encode_itypes t1s = encode_itypes t2s ⇔ t1s = t2s)
+  (∀t1 t2. encode_itype t1 = encode_itype t2 ⇔ t1 = t2)
 Proof
-  rw[] >> eq_tac >> rw[] >>
+  rw[EQ_IMP_THM] >>
   irule $ iffLR SOME_11 >> once_rewrite_tac[GSYM decode_encode] >> simp[]
 QED
 
@@ -258,393 +210,6 @@ Proof
   every_case_tac >> gvs[encode_itype_injective]
 QED
 
-Theorem encode_unify_lemma:
-  ∀s t1 t2 s' t1' t2'.
-    s = encode_itype o_f s' ∧
-    pure_wfs s' ∧
-    (
-      (t1 = encode_itype t1' ∧ t2 = encode_itype t2') ∨
-      (∃c. t1 = Const c ∧ t2 = Const c ∧ t1' = t2') ∨
-      (∃c ts1 ts2.
-        t1 = Pair (Const c) (encode_itypes ts1) ∧
-        t2 = Pair (Const c) (encode_itypes ts2) ∧
-          ((t1' = TypeCons ARB ts1 ∧ t2' = TypeCons ARB ts2) ∨
-           (t1' = Tuple ts1 ∧ t2' = Tuple ts2))) ∨
-      (∃c t11 t12 t21 t22.
-        t1 = Pair (Const c) (Pair (encode_itype t11) (encode_itype t12)) ∧
-        t2 = Pair (Const c) (Pair (encode_itype t21) (encode_itype t22)) ∧
-        t1' = Function t11 t12 ∧ t2' = Function t21 t22) ∨
-      (∃c ta tb.
-        t1 = Pair (Const c) (encode_itype ta) ∧
-        t2 = Pair (Const c) (encode_itype tb) ∧
-        ((t1' = Array ta ∧ t2' = Array tb) ∨
-         (t1' = M ta ∧ t2' = M tb))) ∨
-
-      (∃ts1 ts2.
-        t1 = encode_itypes ts1 ∧
-        t2 = encode_itypes ts2 ∧
-          ((t1' = TypeCons ARB ts1 ∧ t2' = TypeCons ARB ts2) ∨
-           (t1' = Tuple ts1 ∧ t2' = Tuple ts2))) ∨
-      (∃t11 t12 t21 t22.
-        t1 = Pair (encode_itype t11) (encode_itype t12) ∧
-        t2 = Pair (encode_itype t21) (encode_itype t22) ∧
-        t1' = Function t11 t12 ∧ t2' = Function t21 t22) ∨
-      (∃ta tb.
-        t1 = encode_itype ta ∧
-        t2 = encode_itype tb ∧
-          ((t1' = Array ta ∧ t2' = Array tb) ∨
-           (t1' = M ta ∧ t2' = M tb)))
-    )
-  ⇒ unify s t1 t2 = OPTION_MAP ((o_f) encode_itype) (pure_unify s' t1' t2')
-Proof
-  recInduct unify_ind >> simp[] >>
-  rw[pure_unify_def] >> gvs[pure_wfs_def, option_map_case] >>
-  qmatch_assum_abbrev_tac `wfs es`
-  >- (
-    qmatch_goalsub_abbrev_tac `unify es e1 e2` >>
-    Cases_on `unify es e1 e2` >> gvs[combinTheory.o_DEF] >>
-    qsuff_tac `∃s. x = encode_itype o_f s`
-    >- (strip_tac >> rw[GSYM fmap_EQ_THM, decode_encode]) >>
-    pop_assum mp_tac >> simp[Once unify_def] >>
-    Cases_on `walk es e1` >> Cases_on `walk es e2` >> gvs[]
-    >- (
-      unabbrev_all_tac >> rw[]
-      >- (irule_at Any EQ_REFL) >>
-      mp_tac encode_walk >> simp[pure_wfs_def] >>
-      disch_then imp_res_tac >> rgs[] >> rgs[pure_walk_def] >>
-      qmatch_goalsub_abbrev_tac ` _ m |+ (k,v)` >>
-      qmatch_asmsub_abbrev_tac `encode_itype foo = v` >>
-      qexists_tac `m |+ (k,foo)` >> rw[]
-      )
-    >- (
-      unabbrev_all_tac >> rw[] >>
-      mp_tac encode_walk >> simp[pure_wfs_def] >>
-      disch_then imp_res_tac >> rgs[] >> rgs[pure_walk_def] >>
-      qmatch_goalsub_abbrev_tac ` _ m |+ (k,v)` >>
-      qmatch_asmsub_abbrev_tac `encode_itype foo = v` >>
-      qexists_tac `m |+ (k,foo)` >> rw[]
-      )
-    >- (
-      unabbrev_all_tac >> rw[] >>
-      mp_tac encode_walk >> simp[pure_wfs_def] >>
-      disch_then imp_res_tac >> rgs[] >> rgs[pure_walk_def] >>
-      qmatch_goalsub_abbrev_tac ` _ m |+ (k,v)` >>
-      qmatch_asmsub_abbrev_tac `encode_itype foo = v` >>
-      qexists_tac `m |+ (k,foo)` >> rw[]
-      )
-    >- (
-      unabbrev_all_tac >> rw[] >>
-      mp_tac encode_walk >> simp[pure_wfs_def] >>
-      disch_then imp_res_tac >> rgs[] >> rgs[pure_walk_def] >>
-      qmatch_goalsub_abbrev_tac ` _ m |+ (k,v)` >>
-      qmatch_asmsub_abbrev_tac `encode_itype foo = v` >>
-      qexists_tac `m |+ (k,foo)` >> rw[]
-      )
-    >- (
-      rw[] >> gvs[] >>
-      qmatch_assum_rename_tac `walk es e1 = Pair t1a t1d` >>
-      qmatch_assum_rename_tac `walk es e2 = Pair t2a t2d` >>
-      `Pair t1a t1d = encode_itype (pure_walk s' t1')` by
-        metis_tac[encode_walk,pure_wfs_def] >>
-      `Pair t2a t2d = encode_itype (pure_walk s' t2')` by
-        metis_tac[encode_walk,pure_wfs_def] >>
-      `wfs sx` by metis_tac[unify_unifier] >>
-      `∀c1 c2.
-        ((t1a = Const c1 ∧ t2a = Const c2) ∨
-         (t2d = Const c1 ∧ t2d = Const c2)) ⇒ c1 = c2` by (
-          rw[] >> ntac 2 $ qpat_x_assum `unify _ _ _ = _` mp_tac >>
-          simp[Once unify_def] >> strip_tac >> simp[Once unify_def]) >>
-      pop_assum mp_tac >> simp[DISJ_IMP_THM, FORALL_AND_THM] >> strip_tac >>
-      qspecl_then [`pure_walk s' t1'`,`t1a`,`t1d`] mp_tac encode_pair_cases >>
-      qspecl_then [`pure_walk s' t2'`,`t2a`,`t2d`] mp_tac encode_pair_cases >>
-      simp[] >> strip_tac >> strip_tac >> gvs[] >>
-      rpt $ qpat_x_assum `Pair _ _ = _` $ assume_tac o GSYM
-      >- (
-        last_x_assum $
-          qspecl_then[`s'`,`TypeCons ARB ts'`,`TypeCons ARB ts`] mp_tac >>
-        simp[] >> CASE_TAC >> simp[] >> metis_tac[o_f_o_f]
-        )
-      >- (
-        last_x_assum $
-          qspecl_then[`s'`,`Tuple ts'`,`Tuple ts`] mp_tac >>
-        simp[] >> CASE_TAC >> simp[] >> metis_tac[o_f_o_f]
-        )
-      >- (
-        last_x_assum $
-          qspecl_then[`s'`,`Function it1' it2'`,`Function it1 it2`] mp_tac >>
-        simp[encode_itype_def] >>
-        CASE_TAC >> simp[] >> metis_tac[o_f_o_f]
-        )
-      >- (
-        last_x_assum $
-          qspecl_then[`s'`,`Array t'`,`Array t`] mp_tac >>
-        simp[encode_itype_def] >> CASE_TAC >> simp[] >> metis_tac[o_f_o_f]
-        )
-      >- (
-        last_x_assum $
-          qspecl_then[`s'`,`M t'`,`M t`] mp_tac >>
-        simp[encode_itype_def] >> CASE_TAC >> simp[] >> metis_tac[o_f_o_f]
-        )
-      )
-    >- (
-      unabbrev_all_tac >> rw[] >>
-      mp_tac encode_walk >> simp[pure_wfs_def] >>
-      disch_then imp_res_tac >> rgs[] >> rgs[pure_walk_def] >>
-      qmatch_goalsub_abbrev_tac ` _ m |+ (k,v)` >>
-      qmatch_asmsub_abbrev_tac `encode_itype foo = v` >>
-      qexists_tac `m |+ (k,foo)` >> rw[]
-      )
-    >- (unabbrev_all_tac >> rw[] >> irule_at Any EQ_REFL)
-    )
-  >- simp[decode_encode, SF ETA_ss, combinTheory.o_DEF]
-  >- (unabbrev_all_tac >> rw[Once unify_def])
-  >- (unabbrev_all_tac >> rw[Once unify_def])
-  >- (unabbrev_all_tac >> rw[Once unify_def])
-  >- (unabbrev_all_tac >> rw[Once unify_def])
-  >- (unabbrev_all_tac >> rw[Once unify_def])
-  >- (
-    simp[encode_itype_def] >>
-    simp[Once unify_def, SimpRHS] >> CASE_TAC >> pop_assum mp_tac >>
-    Cases_on `ts1` >> Cases_on `ts2` >> simp[encode_itype_def, Once unify_def]
-    >- (
-      rw[Abbr `es`] >>
-      simp[o_f_o_f, combinTheory.o_DEF, decode_encode, SF ETA_ss]
-      ) >>
-    rw[] >> gvs[encode_itype_def] >>
-    first_x_assum $ qspecl_then [`s'`,`h`,`h'`] mp_tac >> simp[] >> rw[] >>
-    `wfs sx` by metis_tac[unify_unifier] >>
-    qabbrev_tac `dx = decode_utype o_f sx` >> simp[combinTheory.o_DEF] >>
-    `sx = encode_itype o_f THE o_f dx` by rw[Abbr `dx`] >>
-    first_x_assum $ qspecl_then
-      [`THE o_f dx`,`TypeCons ARB t`,`TypeCons ARB t'`] mp_tac >>
-    pop_assum $ SUBST1_TAC o GSYM >> simp[encode_itype_def] >>
-    simp[Once unify_def, combinTheory.o_DEF]
-    )
-  >- (
-    simp[encode_itype_def] >>
-    simp[Once unify_def, SimpRHS] >> CASE_TAC >> pop_assum mp_tac >>
-    Cases_on `ts1` >> Cases_on `ts2` >> simp[encode_itype_def, Once unify_def]
-    >- (
-      rw[Abbr `es`] >>
-      simp[o_f_o_f, combinTheory.o_DEF, decode_encode, SF ETA_ss]
-      ) >>
-    rw[] >> gvs[encode_itype_def] >>
-    first_x_assum $ qspecl_then [`s'`,`h`,`h'`] mp_tac >> simp[] >> rw[] >>
-    `wfs sx` by metis_tac[unify_unifier] >>
-    qabbrev_tac `dx = decode_utype o_f sx` >> simp[combinTheory.o_DEF] >>
-    `sx = encode_itype o_f THE o_f dx` by rw[Abbr `dx`] >>
-    first_x_assum $ qspecl_then [`THE o_f dx`,`Tuple t`,`Tuple t'`] mp_tac >>
-    pop_assum $ SUBST1_TAC o GSYM >> simp[encode_itype_def] >>
-    simp[Once unify_def, combinTheory.o_DEF]
-    )
-  >- (
-    simp[encode_itype_def] >>
-    simp[Once unify_def, SimpRHS] >> CASE_TAC >> pop_assum mp_tac >>
-    simp[Once unify_def] >> rw[] >> gvs[encode_itype_def] >>
-    first_x_assum $ qspecl_then [`s'`,`t11`,`t21`] mp_tac >> simp[] >> rw[] >>
-    `wfs sx` by metis_tac[unify_unifier] >>
-    qabbrev_tac `dx = decode_utype o_f sx` >> simp[combinTheory.o_DEF] >>
-    `sx = encode_itype o_f THE o_f dx` by rw[Abbr `dx`] >>
-    first_x_assum $ qspecl_then [`THE o_f dx`,`t12`,`t22`] mp_tac >>
-    pop_assum $ SUBST1_TAC o GSYM >> simp[] >>
-    simp[Once unify_def, combinTheory.o_DEF]
-    )
-  >- (
-    simp[encode_itype_def] >>
-    simp[Once unify_def, SimpRHS] >>
-    qmatch_goalsub_abbrev_tac `unify es e1 e2` >> CASE_TAC >>
-    qsuff_tac `∃s. x = encode_itype o_f s`
-    >- (strip_tac >> rw[GSYM fmap_EQ_THM, decode_encode]) >>
-    pop_assum mp_tac >> simp[Once unify_def] >>
-    Cases_on `walk es e1` >> Cases_on `walk es e2` >> gvs[]
-    >- (
-      unabbrev_all_tac >> rw[]
-      >- (irule_at Any EQ_REFL) >>
-      mp_tac encode_walk >> simp[pure_wfs_def] >>
-      disch_then imp_res_tac >> rgs[] >> rgs[pure_walk_def] >>
-      qmatch_goalsub_abbrev_tac ` _ m |+ (k,v)` >>
-      qmatch_asmsub_abbrev_tac `encode_itype foo = v` >>
-      qexists_tac `m |+ (k,foo)` >> rw[]
-      )
-    >- (
-      unabbrev_all_tac >> rw[] >>
-      mp_tac encode_walk >> simp[pure_wfs_def] >>
-      disch_then imp_res_tac >> rgs[] >> rgs[pure_walk_def] >>
-      qmatch_goalsub_abbrev_tac ` _ m |+ (k,v)` >>
-      qmatch_asmsub_abbrev_tac `encode_itype foo = v` >>
-      qexists_tac `m |+ (k,foo)` >> rw[]
-      )
-    >- (
-      unabbrev_all_tac >> rw[] >>
-      mp_tac encode_walk >> simp[pure_wfs_def] >>
-      disch_then imp_res_tac >> rgs[] >> rgs[pure_walk_def] >>
-      qmatch_goalsub_abbrev_tac ` _ m |+ (k,v)` >>
-      qmatch_asmsub_abbrev_tac `encode_itype foo = v` >>
-      qexists_tac `m |+ (k,foo)` >> rw[]
-      )
-    >- (
-      unabbrev_all_tac >> rw[] >>
-      mp_tac encode_walk >> simp[pure_wfs_def] >>
-      disch_then imp_res_tac >> rgs[] >> rgs[pure_walk_def] >>
-      qmatch_goalsub_abbrev_tac ` _ m |+ (k,v)` >>
-      qmatch_asmsub_abbrev_tac `encode_itype foo = v` >>
-      qexists_tac `m |+ (k,foo)` >> rw[]
-      )
-    >- (
-      rw[] >> gvs[] >>
-      qmatch_assum_rename_tac `walk es e1 = Pair t1a t1d` >>
-      qmatch_assum_rename_tac `walk es e2 = Pair t2a t2d` >>
-      `Pair t1a t1d = encode_itype (pure_walk s' ta)` by
-        metis_tac[encode_walk,pure_wfs_def] >>
-      `Pair t2a t2d = encode_itype (pure_walk s' tb)` by
-        metis_tac[encode_walk,pure_wfs_def] >>
-      `wfs sx` by metis_tac[unify_unifier] >>
-      `∀c1 c2.
-        ((t1a = Const c1 ∧ t2a = Const c2) ∨
-         (t2d = Const c1 ∧ t2d = Const c2)) ⇒ c1 = c2` by (
-          rw[] >> ntac 2 $ qpat_x_assum `unify _ _ _ = _` mp_tac >>
-          simp[Once unify_def] >> strip_tac >> simp[Once unify_def]) >>
-      pop_assum mp_tac >> simp[DISJ_IMP_THM, FORALL_AND_THM] >> strip_tac >>
-      qspecl_then [`pure_walk s' ta`,`t1a`,`t1d`] mp_tac encode_pair_cases >>
-      qspecl_then [`pure_walk s' tb`,`t2a`,`t2d`] mp_tac encode_pair_cases >>
-      simp[] >> strip_tac >> strip_tac >> gvs[] >>
-      rpt $ qpat_x_assum `Pair _ _ = _` $ assume_tac o GSYM
-      >- (
-        last_x_assum $
-          qspecl_then[`s'`,`TypeCons ARB ts'`,`TypeCons ARB ts`] mp_tac >>
-        simp[] >> CASE_TAC >> simp[] >> metis_tac[o_f_o_f]
-        )
-      >- (
-        last_x_assum $
-          qspecl_then[`s'`,`Tuple ts'`,`Tuple ts`] mp_tac >>
-        simp[] >> CASE_TAC >> simp[] >> metis_tac[o_f_o_f]
-        )
-      >- (
-        last_x_assum $
-          qspecl_then[`s'`,`Function it1' it2'`,`Function it1 it2`] mp_tac >>
-        simp[encode_itype_def] >>
-        CASE_TAC >> simp[] >> metis_tac[o_f_o_f]
-        )
-      >- (
-        last_x_assum $
-          qspecl_then[`s'`,`Array t'`,`Array t`] mp_tac >>
-        simp[encode_itype_def] >> CASE_TAC >> simp[] >> metis_tac[o_f_o_f]
-        )
-      >- (
-        last_x_assum $
-          qspecl_then[`s'`,`M t'`,`M t`] mp_tac >>
-        simp[encode_itype_def] >> CASE_TAC >> simp[] >> metis_tac[o_f_o_f]
-        )
-      )
-    >- (
-      unabbrev_all_tac >> rw[] >>
-      mp_tac encode_walk >> simp[pure_wfs_def] >>
-      disch_then imp_res_tac >> rgs[] >> rgs[pure_walk_def] >>
-      qmatch_goalsub_abbrev_tac ` _ m |+ (k,v)` >>
-      qmatch_asmsub_abbrev_tac `encode_itype foo = v` >>
-      qexists_tac `m |+ (k,foo)` >> rw[]
-      )
-    >- (unabbrev_all_tac >> rw[] >> irule_at Any EQ_REFL)
-    )
-  >- (
-    simp[encode_itype_def] >>
-    simp[Once unify_def, SimpRHS] >>
-    qmatch_goalsub_abbrev_tac `unify es e1 e2` >> CASE_TAC >>
-    qsuff_tac `∃s. x = encode_itype o_f s`
-    >- (strip_tac >> rw[GSYM fmap_EQ_THM, decode_encode]) >>
-    pop_assum mp_tac >> simp[Once unify_def] >>
-    Cases_on `walk es e1` >> Cases_on `walk es e2` >> gvs[]
-    >- (
-      unabbrev_all_tac >> rw[]
-      >- (irule_at Any EQ_REFL) >>
-      mp_tac encode_walk >> simp[pure_wfs_def] >>
-      disch_then imp_res_tac >> rgs[] >> rgs[pure_walk_def] >>
-      qmatch_goalsub_abbrev_tac ` _ m |+ (k,v)` >>
-      qmatch_asmsub_abbrev_tac `encode_itype foo = v` >>
-      qexists_tac `m |+ (k,foo)` >> rw[]
-      )
-    >- (
-      unabbrev_all_tac >> rw[] >>
-      mp_tac encode_walk >> simp[pure_wfs_def] >>
-      disch_then imp_res_tac >> rgs[] >> rgs[pure_walk_def] >>
-      qmatch_goalsub_abbrev_tac ` _ m |+ (k,v)` >>
-      qmatch_asmsub_abbrev_tac `encode_itype foo = v` >>
-      qexists_tac `m |+ (k,foo)` >> rw[]
-      )
-    >- (
-      unabbrev_all_tac >> rw[] >>
-      mp_tac encode_walk >> simp[pure_wfs_def] >>
-      disch_then imp_res_tac >> rgs[] >> rgs[pure_walk_def] >>
-      qmatch_goalsub_abbrev_tac ` _ m |+ (k,v)` >>
-      qmatch_asmsub_abbrev_tac `encode_itype foo = v` >>
-      qexists_tac `m |+ (k,foo)` >> rw[]
-      )
-    >- (
-      unabbrev_all_tac >> rw[] >>
-      mp_tac encode_walk >> simp[pure_wfs_def] >>
-      disch_then imp_res_tac >> rgs[] >> rgs[pure_walk_def] >>
-      qmatch_goalsub_abbrev_tac ` _ m |+ (k,v)` >>
-      qmatch_asmsub_abbrev_tac `encode_itype foo = v` >>
-      qexists_tac `m |+ (k,foo)` >> rw[]
-      )
-    >- (
-      rw[] >> gvs[] >>
-      qmatch_assum_rename_tac `walk es e1 = Pair t1a t1d` >>
-      qmatch_assum_rename_tac `walk es e2 = Pair t2a t2d` >>
-      `Pair t1a t1d = encode_itype (pure_walk s' ta)` by
-        metis_tac[encode_walk,pure_wfs_def] >>
-      `Pair t2a t2d = encode_itype (pure_walk s' tb)` by
-        metis_tac[encode_walk,pure_wfs_def] >>
-      `wfs sx` by metis_tac[unify_unifier] >>
-      `∀c1 c2.
-        ((t1a = Const c1 ∧ t2a = Const c2) ∨
-         (t2d = Const c1 ∧ t2d = Const c2)) ⇒ c1 = c2` by (
-          rw[] >> ntac 2 $ qpat_x_assum `unify _ _ _ = _` mp_tac >>
-          simp[Once unify_def] >> strip_tac >> simp[Once unify_def]) >>
-      pop_assum mp_tac >> simp[DISJ_IMP_THM, FORALL_AND_THM] >> strip_tac >>
-      qspecl_then [`pure_walk s' ta`,`t1a`,`t1d`] mp_tac encode_pair_cases >>
-      qspecl_then [`pure_walk s' tb`,`t2a`,`t2d`] mp_tac encode_pair_cases >>
-      simp[] >> strip_tac >> strip_tac >> gvs[] >>
-      rpt $ qpat_x_assum `Pair _ _ = _` $ assume_tac o GSYM
-      >- (
-        last_x_assum $
-          qspecl_then[`s'`,`TypeCons ARB ts'`,`TypeCons ARB ts`] mp_tac >>
-        simp[] >> CASE_TAC >> simp[] >> metis_tac[o_f_o_f]
-        )
-      >- (
-        last_x_assum $
-          qspecl_then[`s'`,`Tuple ts'`,`Tuple ts`] mp_tac >>
-        simp[] >> CASE_TAC >> simp[] >> metis_tac[o_f_o_f]
-        )
-      >- (
-        last_x_assum $
-          qspecl_then[`s'`,`Function it1' it2'`,`Function it1 it2`] mp_tac >>
-        simp[encode_itype_def] >>
-        CASE_TAC >> simp[] >> metis_tac[o_f_o_f]
-        )
-      >- (
-        last_x_assum $
-          qspecl_then[`s'`,`Array t'`,`Array t`] mp_tac >>
-        simp[encode_itype_def] >> CASE_TAC >> simp[] >> metis_tac[o_f_o_f]
-        )
-      >- (
-        last_x_assum $
-          qspecl_then[`s'`,`M t'`,`M t`] mp_tac >>
-        simp[encode_itype_def] >> CASE_TAC >> simp[] >> metis_tac[o_f_o_f]
-        )
-      )
-    >- (
-      unabbrev_all_tac >> rw[] >>
-      mp_tac encode_walk >> simp[pure_wfs_def] >>
-      disch_then imp_res_tac >> rgs[] >> rgs[pure_walk_def] >>
-      qmatch_goalsub_abbrev_tac ` _ m |+ (k,v)` >>
-      qmatch_asmsub_abbrev_tac `encode_itype foo = v` >>
-      qexists_tac `m |+ (k,foo)` >> rw[]
-      )
-    >- (unabbrev_all_tac >> rw[] >> irule_at Any EQ_REFL)
-    )
-QED
-
 Theorem encode_unify:
   ∀s t1 t2 s' t1' t2'.
     s = encode_itype o_f s' ∧
@@ -653,7 +218,10 @@ Theorem encode_unify:
     pure_wfs s'
   ⇒ unify s t1 t2 = OPTION_MAP ((o_f) encode_itype) (pure_unify s' t1' t2')
 Proof
-  metis_tac[encode_unify_lemma]
+  simp[option_map_case,pure_unify_def] >>
+  rw[] >>
+  CASE_TAC >>
+  simp[o_f_o_f,combinTheory.o_DEF,encode_decode]
 QED
 
 Theorem encode_unify_alt:
@@ -661,7 +229,7 @@ Theorem encode_unify_alt:
     unify (encode_itype o_f s) (encode_itype t1) (encode_itype t2) =
     OPTION_MAP ((o_f) encode_itype) (pure_unify s t1 t2)
 Proof
-  metis_tac[encode_unify_lemma]
+  metis_tac[encode_unify]
 QED
 
 Theorem wfs_unify:
@@ -670,444 +238,185 @@ Proof
   metis_tac[unify_unifier]
 QED
 
-Theorem pure_unifyl:
-  ∀s l1 l2.
-    pure_wfs s ⇒
-      pure_unifyl s l1 l2 =
-        OPTION_MAP ((o_f) (THE o decode_utype)) $
-          unify (encode_itype o_f s) (encode_itypes l1) (encode_itypes l2)
-Proof
-  Induct_on `l1` >> Cases_on `l2` >> rw[pure_unifyl_def, encode_itype_def] >>
-  imp_res_tac pure_wfs_def >>
-  gvs[OPTION_MAP_CASE, combinTheory.o_DEF, decode_encode]
-  >- rw[Once unify_def] >- rw[Once unify_def] >>
-  rw[Once unify_def] >> rw[pure_unify_def, combinTheory.o_DEF] >>
-  simp[OPTION_MAP_CASE, combinTheory.o_DEF] >>
-  CASE_TAC >> simp[] >>
-  imp_res_tac encode_unify_alt >> gvs[combinTheory.o_DEF, decode_encode] >>
-  last_x_assum irule >> rgs[pure_wfs_def, pure_unify_def] >>
-  irule wfs_unify >> goal_assum drule >>
-  irule_at Any EQ_TRANS >> pop_assum $ irule_at Any >> simp[PULL_EXISTS] >>
-  goal_assum drule >> simp[]
-QED
-
 Theorem pure_unify:
   ∀t1 t2 s.
     pure_wfs s ⇒
     pure_unify s t1 t2 =
       case (pure_walk s t1, pure_walk s t2) of
-      | (CVar v1 ts1, CVar v2 ts2) =>
-          SOME (if v1 = v2 then s else s |+ (v1, CVar v2))
-      | (CVar v1 ts1, t2) => let (tc2,tl2) = split_Cons t2 in
-          OPTION_BIND (pure_unifyl (LASTN (LENGTH tl2) ts1) tl2)
-          (λs'. pure_ext_s_check s' v1 tc2)
-      | (t1, CVar v2 ts2) => pure_ext_s_check s v2 t1
-      | (TypeCons c1 ts1, TypeCons c2 ts2) =>
-          if c1 = c2 then pure_unifyl s ts1 ts2 else NONE
-      | (DBVarCons db1 ts1, DBVarCons db2 ts2) =>
-          if db1 = db2 then pure_unifyl s ts1 ts2 else NONE
-      | (PrimTy pty1, PrimTy pty2) => if pty1 = pty2 then SOME s else NONE
-      | (Exception, Exception) => SOME s
+      | (iCVar v1, iCVar v2) =>
+          SOME (if v1 = v2 then s else s |+ (v1, iCVar v2))
+      | (iCVar v1, t2) => pure_ext_s_check s v1 t2
+      | (t1, iCVar v2) => pure_ext_s_check s v2 t1
+      | (iCons l1 r1,iCons l2 r2) =>
+          OPTION_BIND (pure_unify s l1 l2)
+            ( λs'. pure_unify s' r1 r2)
+      | (iAtom a1,iAtom a2) =>
+          if a1 = a2 then SOME s else NONE
       | (t1, t2) => NONE
 Proof
   rw[pure_unify_def] >> imp_res_tac pure_wfs_def >>
   rw [Once unify_def, pure_walk_def] >>
   Cases_on `t1` >> Cases_on `t2` >>
   rw[encode_itype_def, decode_utype_def, option_map_case, option_bind_case,
-     combinTheory.o_DEF, decode_encode, encode_vwalk, pure_unifyl, pure_oc_lemma]
+     combinTheory.o_DEF, decode_encode, encode_vwalk]
   >- (
-    Cases_on `pure_vwalk s n'` >> gvs[decode_encode] >>
-    simp[encode_itype_def] >> rw[] >>
-    simp[pure_ext_s_check, Once pure_oc, pure_walk, decode_utype_def] >>
-    gvs[combinTheory.o_DEF, decode_encode]
+    Cases_on `pure_vwalk s n` >>
+    gvs[decode_encode,encode_itype_def] >>
+    rw[pure_ext_s_check, Once pure_oc, pure_walk,
+      decode_utype_def,combinTheory.o_DEF,
+      decode_encode,encode_decode]
     )
   >- (
-    Cases_on `pure_vwalk s n` >> gvs[decode_encode] >>
-    simp[encode_itype_def] >> rw[] >>
-    simp[pure_ext_s_check, Once pure_oc, pure_walk, decode_utype_def] >>
-    gvs[combinTheory.o_DEF, decode_encode]
+    ntac 2 CASE_TAC >>
+    simp[o_f_o_f,encode_decode,combinTheory.o_DEF]
     )
   >- (
-    Cases_on `pure_vwalk s n` >> gvs[decode_encode] >>
-    simp[encode_itype_def] >> rw[] >>
-    simp[pure_ext_s_check, Once pure_oc, pure_walk, decode_utype_def] >>
-    gvs[combinTheory.o_DEF, decode_encode]
-    )
-  >- simp[Once unify_def]
-  >- simp[Once unify_def]
-  >- simp[Once unify_def]
-  >- simp[Once unify_def]
-  >- simp[Once unify_def]
-  >- (
-    simp[Once unify_def] >>
-    Cases_on `pure_vwalk s n'` >> gvs[decode_encode] >>
-    simp[encode_itype_def] >> rw[] >>
-    simp[pure_ext_s_check, Once pure_oc, pure_walk, decode_utype_def, pure_oc_def] >>
-    gvs[combinTheory.o_DEF, decode_encode]
-    )
-  >- simp[Once unify_def]
-  >- simp[Once unify_def]
-  >- simp[Once unify_def]
-  >- simp[Once unify_def]
-  >- (
-    simp[Once unify_def] >>
-    Cases_on `pure_vwalk s n` >> gvs[decode_encode] >>
-    simp[encode_itype_def] >> rw[] >>
-    simp[pure_ext_s_check, Once pure_oc, pure_walk, decode_utype_def, pure_oc_def] >>
-    gvs[combinTheory.o_DEF, decode_encode]
-    )
-  >- simp[Once unify_def]
-  >- simp[Once unify_def]
-  >- (
-    simp[Once unify_def, SimpRHS] >> simp[Once unify_def, option_bind_case] >>
-    CASE_TAC >> drule_all wfs_unify >> strip_tac >>
-    simp[Once unify_def, SimpRHS, option_bind_case] >>
-    CASE_TAC >> drule_all wfs_unify >> strip_tac >> simp[Once unify_def]
-    )
-  >- simp[Once unify_def]
-  >- simp[Once unify_def]
-  >- (
-    ntac 2 $ simp[Once unify_def, option_bind_case] >>
-    Cases_on `pure_vwalk s n` >> gvs[decode_encode] >>
-    simp[encode_itype_def] >> rw[]
+    Cases_on `pure_vwalk s n` >>
+    gvs[decode_encode,encode_itype_def]
     >- (
-      simp[Once unify_def, option_bind_case] >>
-      CASE_TAC >> drule_all wfs_unify >> strip_tac >>
-      simp[Once unify_def, SimpRHS, option_bind_case] >>
-      CASE_TAC >> drule_all wfs_unify >> strip_tac >> simp[Once unify_def]
+      ntac 2 CASE_TAC >>
+      simp[o_f_o_f,combinTheory.o_DEF,encode_decode]
       ) >>
-    simp[pure_ext_s_check, Once pure_oc, pure_walk, decode_utype_def, pure_oc_def] >>
-    gvs[combinTheory.o_DEF, decode_encode]
-    )
-  >- simp[Once unify_def]
-  >- simp[Once unify_def]
-  >- simp[Once unify_def]
-  >- simp[Once unify_def]
-  >- (
-    simp[Once unify_def] >>
-    Cases_on `pure_vwalk s n` >> gvs[decode_encode] >>
-    simp[encode_itype_def] >> rw[] >>
-    simp[pure_ext_s_check, Once pure_oc, pure_walk, decode_utype_def, pure_oc_def] >>
-    gvs[combinTheory.o_DEF, decode_encode]
-    )
-  >- simp[Once unify_def]
-  >- simp[Once unify_def]
-  >- simp[Once unify_def]
-  >- simp[Once unify_def]
-  >- (
-    simp[Once unify_def] >>
-    Cases_on `pure_vwalk s n` >> gvs[decode_encode] >>
-    simp[encode_itype_def] >> rw[] >>
-    simp[pure_ext_s_check, Once pure_oc, pure_walk, decode_utype_def, pure_oc_def] >>
-    gvs[combinTheory.o_DEF, decode_encode]
+    simp[pure_ext_s_check,Once pure_oc,pure_walk] >>
+    simp[pure_oc_def] >>
+    IF_CASES_TAC >>
+    simp[combinTheory.o_DEF,decode_encode,decode_utype_def]
     )
   >- (
-    simp[Once unify_def] >>
-    Cases_on `pure_vwalk s n` >> gvs[decode_encode] >>
-    simp[encode_itype_def] >> rw[] >>
-    simp[pure_ext_s_check, Once pure_oc, pure_walk, decode_utype_def, pure_oc_def] >>
-    gvs[combinTheory.o_DEF, decode_encode]
-    )
-  >- (
-    simp[Once unify_def] >>
-    Cases_on `pure_vwalk s n` >> gvs[decode_encode] >>
-    simp[encode_itype_def] >> rw[] >>
-    simp[pure_ext_s_check, Once pure_oc, pure_walk, decode_utype_def, pure_oc_def] >>
-    gvs[combinTheory.o_DEF, decode_encode]
-    )
-  >- (
-    simp[Once unify_def] >>
-    Cases_on `pure_vwalk s n` >> gvs[decode_encode] >>
-    simp[encode_itype_def] >> rw[] >>
-    simp[pure_ext_s_check, Once pure_oc, pure_walk, decode_utype_def, pure_oc_def] >>
-    gvs[combinTheory.o_DEF, decode_encode]
-    )
-  >- (
-    simp[Once unify_def] >>
-    Cases_on `pure_vwalk s n` >> gvs[decode_encode] >>
-    simp[encode_itype_def] >> rw[] >>
-    simp[pure_ext_s_check, Once pure_oc, pure_walk, decode_utype_def, pure_oc_def] >>
-    gvs[combinTheory.o_DEF, decode_encode]
-    )
-  >- (
-    simp[Once unify_def] >>
-    Cases_on `pure_vwalk s n` >> gvs[decode_encode] >>
-    simp[encode_itype_def] >> rw[] >>
-    simp[pure_ext_s_check, Once pure_oc, pure_walk, decode_utype_def, pure_oc_def] >>
-    gvs[combinTheory.o_DEF, decode_encode]
-    )
-  >- (
-    simp[Once unify_def] >>
-    Cases_on `pure_vwalk s n` >> gvs[decode_encode] >>
-    simp[Once unify_def, option_bind_case] >>
-    simp[encode_itype_def] >> rw[]
+    Cases_on `pure_vwalk s n` >>
+    gvs[decode_encode,encode_itype_def]
     >- (
-      simp[Once unify_def, option_bind_case] >>
-      CASE_TAC >> drule_all wfs_unify >> strip_tac >>
-      simp[Once unify_def, SimpRHS, option_bind_case] >>
-      CASE_TAC >> drule_all wfs_unify >> strip_tac >> simp[Once unify_def]
+      CASE_TAC >>
+      simp[o_f_o_f,combinTheory.o_DEF,decode_encode]
       ) >>
-    simp[pure_ext_s_check, Once pure_oc, pure_walk, decode_utype_def, pure_oc_def] >>
-    gvs[combinTheory.o_DEF, decode_encode]
-    )
+    simp[o_f_o_f,combinTheory.o_DEF,decode_encode,
+      pure_ext_s_check,decode_utype_def,
+      Once pure_oc,pure_walk]
+  )
   >- (
-    simp[Once unify_def] >>
-    Cases_on `pure_vwalk s n` >> gvs[decode_encode] >>
-    simp[encode_itype_def] >> rw[] >>
-    simp[pure_ext_s_check, Once pure_oc, pure_walk, decode_utype_def, pure_oc_def] >>
-    gvs[combinTheory.o_DEF, decode_encode]
-    )
-  >- (
-    simp[Once unify_def] >>
-    Cases_on `pure_vwalk s n` >> gvs[decode_encode] >>
-    simp[encode_itype_def] >> rw[] >>
-    simp[pure_ext_s_check, Once pure_oc, pure_walk, decode_utype_def, pure_oc_def] >>
-    gvs[combinTheory.o_DEF, decode_encode]
-    ) >>
-  Cases_on `pure_vwalk s n` >> gvs[decode_encode] >>
-  simp[encode_itype_def] >> rw[]
-  >- (
-    Cases_on `pure_vwalk s n'` >> gvs[decode_encode] >>
-    simp[encode_itype_def] >> rw[] >>
-    simp[pure_ext_s_check, Once pure_oc, pure_walk, decode_utype_def, pure_oc_def] >>
-    gvs[combinTheory.o_DEF, decode_encode]
-    )
-  >- (
-    Cases_on `pure_vwalk s n'` >> gvs[decode_encode] >>
-    simp[encode_itype_def] >> rw[] >>
-    simp[pure_ext_s_check, Once pure_oc, pure_walk, decode_utype_def, pure_oc_def] >>
-    gvs[combinTheory.o_DEF, decode_encode]
-    )
-  >- (
-    Cases_on `pure_vwalk s n'` >> gvs[decode_encode] >>
-    simp[encode_itype_def] >> rw[] >>
-    simp[pure_ext_s_check, Once pure_oc, pure_walk, decode_utype_def, pure_oc_def] >>
-    gvs[combinTheory.o_DEF, decode_encode]
-    )
-  >- (
-    Cases_on `pure_vwalk s n'` >> gvs[decode_encode] >>
-    simp[Once unify_def] >>
-    simp[encode_itype_def] >> rw[] >>
-    simp[pure_ext_s_check, Once pure_oc, pure_walk, decode_utype_def, pure_oc_def] >>
-    gvs[combinTheory.o_DEF, decode_encode, pure_oc_lemma]
-    )
-  >- (
-    Cases_on `pure_vwalk s n'` >> gvs[decode_encode] >>
-    simp[Once unify_def] >>
-    simp[encode_itype_def] >> rw[] >>
-    simp[pure_ext_s_check, Once pure_oc, pure_walk, decode_utype_def, pure_oc_def] >>
-    gvs[combinTheory.o_DEF, decode_encode, pure_oc_lemma]
-    )
-  >- (
-    Cases_on `pure_vwalk s n'` >> gvs[decode_encode] >>
-    ntac 2 $ simp[Once unify_def, option_bind_case] >>
-    simp[encode_itype_def] >> rw[]
+    Cases_on `pure_vwalk s n` >>
+    gvs[decode_encode,encode_itype_def]
     >- (
-      simp[Once unify_def, option_bind_case] >>
-      CASE_TAC >> drule_all wfs_unify >> strip_tac >>
-      simp[Once unify_def, SimpRHS, option_bind_case] >>
-      CASE_TAC >> drule_all wfs_unify >> strip_tac >> simp[Once unify_def]
+      ntac 2 CASE_TAC >>
+      simp[o_f_o_f,combinTheory.o_DEF,encode_decode]
       ) >>
-    simp[pure_ext_s_check, Once pure_oc, pure_walk, decode_utype_def, pure_oc_def] >>
-    gvs[combinTheory.o_DEF, decode_encode]
-    )
+    simp[pure_ext_s_check,Once pure_oc,pure_walk] >>
+    simp[pure_oc_def] >>
+    IF_CASES_TAC >>
+    simp[combinTheory.o_DEF,decode_encode,decode_utype_def]
+  )
   >- (
-    Cases_on `pure_vwalk s n'` >> gvs[decode_encode] >>
-    simp[Once unify_def] >>
-    simp[encode_itype_def] >> rw[] >>
-    simp[pure_ext_s_check, Once pure_oc, pure_walk, decode_utype_def, pure_oc_def] >>
-    gvs[combinTheory.o_DEF, decode_encode, pure_oc_lemma]
-    )
-  >- (
-    Cases_on `pure_vwalk s n'` >> gvs[decode_encode] >>
-    simp[Once unify_def] >>
-    simp[encode_itype_def] >> rw[] >>
-    simp[pure_ext_s_check, Once pure_oc, pure_walk, decode_utype_def, pure_oc_def] >>
-    gvs[combinTheory.o_DEF, decode_encode, pure_oc_lemma]
-    )
-  >- (
-    Cases_on `pure_vwalk s n'` >> gvs[decode_encode] >>
-    simp[Once unify_def] >>
-    simp[encode_itype_def] >> rw[] >>
-    simp[pure_ext_s_check, Once pure_oc, pure_walk, decode_utype_def, pure_oc_def] >>
-    gvs[combinTheory.o_DEF, decode_encode, pure_oc_lemma]
-    )
+    Cases_on `pure_vwalk s n` >>
+    gvs[decode_encode,encode_itype_def] >>
+    Cases_on `pure_vwalk s n'` >>
+    gvs[decode_encode,encode_itype_def,decode_utype_def,
+      o_f_o_f,combinTheory.o_DEF,pure_ext_s_check,
+      Once pure_oc,pure_walk]
+    >- (
+      CASE_TAC >>
+      simp[decode_encode,o_f_o_f,combinTheory.o_DEF]
+      )
+    >- (
+      ntac 2 CASE_TAC >>
+      simp[encode_decode,o_f_o_f,combinTheory.o_DEF]
+      )
+    >- (
+      simp[pure_oc_def] >>
+      CASE_TAC >>
+      simp[decode_encode,o_f_o_f,combinTheory.o_DEF,
+        decode_utype_def]
+      )
+    >- (
+      simp[pure_oc_def] >>
+      CASE_TAC >>
+      simp[decode_encode,o_f_o_f,combinTheory.o_DEF,
+        decode_utype_def]
+      )
+    >- (
+      IF_CASES_TAC >>
+      simp[decode_encode,o_f_o_f,combinTheory.o_DEF,
+        decode_utype_def]
+      )
+  )
+QED
+
+Triviality pure_unify_ind_lemma:
+  ∀P.
+    (∀us ut1 ut2 s t1 t2.
+       us = encode_itype o_f s ∧
+       ut1 = encode_itype t1 ∧
+       ut2 = encode_itype t2 ∧
+      (∀l1 r1 l2 r2 sx.
+       pure_walk s t1 = iCons l1 r1 ∧
+       pure_walk s t2 = iCons l2 r2 ∧
+       pure_unify s l1 l2 = SOME sx
+       ⇒ P sx r1 r2) ∧
+      (∀l1 r1 l2 r2.
+        pure_walk s t1 = iCons l1 r1 ∧
+        pure_walk s t2 = iCons l2 r1
+        ⇒ P s l1 l2) ⇒
+       P s t1 t2)
+  ⇒ ∀us ut1 ut2. ∀s t1 t2.
+    us = encode_itype o_f s ∧
+    ut1 = encode_itype t1 ∧
+    ut2 = encode_itype t2 ∧
+    pure_wfs s ⇒ P s t1 t2
+Proof
+  gen_tac >> strip_tac >>
+  ho_match_mp_tac unify_ind >>
+  rpt strip_tac >>
+  last_x_assum irule >>
+  drule_then assume_tac $ iffLR pure_wfs_def >>
+  fs[encode_walk] >>
+  rw[]
+  >- (first_x_assum irule >> simp[encode_itype_def]) >>
+  last_x_assum irule >>
+  simp[encode_itype_def,encode_unify_alt] >>
+  gvs[pure_unify_def] >>
+  drule_all_then assume_tac wfs_unify >>
+  simp[pure_wfs_def] >>
+  gvs[encode_unify_alt,combinTheory.o_DEF,decode_encode] >>
+  metis_tac[]
 QED
 
 Theorem pure_unify_ind:
-  ∀P0 P1.
+  ∀P.
     (∀s t1 t2.
-      (∀ts1 ts2 c.
-        (pure_walk s t1 = TypeCons c ts1 ∧
-         pure_walk s t2 = TypeCons c ts2) ∨
-        (pure_walk s t1 = Tuple ts1 ∧
-         pure_walk s t2 = Tuple ts2) ∨
-        (∃t11 t12 t21 t22.
-         pure_walk s t1 = Function t11 t12 ∧
-         pure_walk s t2 = Function t21 t22 ∧
-         ts1 = [t11;t12] ∧ ts2 = [t21;t22])
-       ⇒ P1 s ts1 ts2) ∧
-      (∀ta tb.
-        (pure_walk s t1 = Array ta ∧
-         pure_walk s t2 = Array tb) ∨
-        (pure_walk s t1 = M ta ∧
-         pure_walk s t2 = M tb)
-       ⇒ P0 s ta tb)
-     ⇒ P0 s t1 t2) ∧
-    (∀s ts1 ts2.
-      (∀t1 ts1' t2 ts2' s'.
-        ts1 = t1::ts1' ∧ ts2 = t2::ts2' ⇒
-        P0 s t1 t2 ∧ (pure_unify s t1 t2 = SOME s' ⇒ P1 s' ts1' ts2'))
-     ⇒ P1 s ts1 ts2)
-  ⇒ (∀s t1 t2. pure_wfs s ⇒ P0 s t1 t2) ∧
-    (∀s ts1 ts2. pure_wfs s ⇒ P1 s ts1 ts2)
+      (∀l1 r1 l2 r2 sx.
+       pure_walk s t1 = iCons l1 r1 ∧
+       pure_walk s t2 = iCons l2 r2 ∧
+       pure_unify s l1 l2 = SOME sx
+       ⇒ P sx r1 r2) ∧
+      (∀l1 r1 l2 r2.
+        pure_walk s t1 = iCons l1 r1 ∧
+        pure_walk s t2 = iCons l2 r1
+        ⇒ P s l1 l2) ⇒
+       P s t1 t2)
+  ⇒ (∀s t1 t2. pure_wfs s ⇒ P s t1 t2)
 Proof
-  rpt gen_tac >> strip_tac >>
-  (fn qt => qspec_then qt strip_assume_tac unify_ind)
-    `λs t1 t2.
-      (∀us u1 u2.
-        wfs s ∧ s = encode_itype o_f us ∧
-        t1 = encode_itype u1 ∧ t2 = encode_itype u2
-       ⇒ P0 us u1 u2) ∧
-      (∀us tag us1 us2 c.
-        wfs s ∧ s = encode_itype o_f us ∧
-        (c = uTypeCons tag ∨ c = uTuple) ∧
-        t1 = Pair (Const c) (encode_itypes us1) ∧
-        t2 = Pair (Const c) (encode_itypes us2)
-       ⇒ P1 us us1 us2) ∧
-      (∀us u11 u12 u21 u22.
-        wfs s ∧ s = encode_itype o_f us ∧
-        t1 = Pair (Const uFunction) (Pair (encode_itype u11) (encode_itype u12)) ∧
-        t2 = Pair (Const uFunction) (Pair (encode_itype u21) (encode_itype u22))
-       ⇒ P1 us [u11;u12] [u21;u22]) ∧
-      (∀us u1 u2 c.
-        wfs s ∧ s = encode_itype o_f us ∧
-        (c = uArray ∨ c = uM) ∧
-        t1 = Pair (Const c) (encode_itype u1) ∧
-        t2 = Pair (Const c) (encode_itype u2)
-       ⇒ P0 us u1 u2) ∧
-      (∀us v1 u1 v2 u2.
-        wfs s ∧ s = encode_itype o_f us ∧
-        t1 = Pair (encode_itype v1) (encode_itypes u1) ∧
-        t2 = Pair (encode_itype v2) (encode_itypes u2)
-       ⇒ P0 us v1 v2 ∧
-         (∀usx.
-            unify s (encode_itype v1) (encode_itype v2) =
-              SOME (encode_itype o_f usx)
-          ⇒ P1 usx u1 u2)) ∧
-      (∀us v1 u1 v2 u2.
-        wfs s ∧ s = encode_itype o_f us ∧
-        t1 = Pair (encode_itype v1) (encode_itype u1) ∧
-        t2 = Pair (encode_itype v2) (encode_itype u2)
-       ⇒ P0 us v1 v2 ∧
-         (∀usx.
-            unify s (encode_itype v1) (encode_itype v2) =
-              SOME (encode_itype o_f usx)
-          ⇒ P1 usx [u1] [u2]))` >>
-  qmatch_assum_abbrev_tac `P ⇒ Q` >> qsuff_tac `P`
-  >- (
-    strip_tac >> `Q` by res_tac >> pop_assum mp_tac >>
-    unabbrev_all_tac >> rpt $ pop_assum kall_tac >>
-    CONV_TAC (DEPTH_CONV BETA_CONV) >> strip_tac >> rw[] >>
-    gvs[encode_itype_injective, encode_itype_o_f_injective, pure_wfs_def]
-    ) >>
-  qpat_x_assum `P ⇒ Q` kall_tac >> unabbrev_all_tac >>
-  CONV_TAC (DEPTH_CONV BETA_CONV) >>
-  rpt gen_tac >> strip_tac >> rpt conj_tac
-  >- (
-    rw[] >> first_x_assum irule >> rw[] >>
-    fs[encode_walk, encode_itype_def, pure_wfs_def,
-       encode_itype_injective, encode_itype_o_f_injective] >>
-    last_x_assum irule >> rpt gen_tac >> strip_tac >>
-    gvs[encode_itype_def, encode_itype_injective] >>
-    gvs[SRULE [pure_wfs_def] encode_unify]
-    )
-  >- (
-    rw[] >> first_x_assum irule >> rw[] >>
-    fs[encode_itype_def, encode_itype_injective, encode_itype_o_f_injective] >>
-    first_x_assum irule >> simp[pure_wfs_def, encode_unify_alt]
-    )
-  >- (
-    rw[] >> first_x_assum irule >> rw[] >>
-    fs[encode_itype_def, encode_itype_injective, encode_itype_o_f_injective] >>
-    first_x_assum irule >> simp[pure_wfs_def, encode_unify_alt]
-    )
-  >- (rpt gen_tac >> strip_tac >> rw[])
-  >- (
-    rw[] >> first_x_assum match_mp_tac >> imp_res_tac wfs_unify >>
-    fs[encode_itype_injective, encode_itype_o_f_injective] >>
-    rw[] >> fs[encode_itype_def, encode_itype_injective] >>
-    simp[pure_wfs_def, encode_unify_alt]
-    )
-  >- (
-    rw[] >> first_assum irule >> imp_res_tac wfs_unify >>
-    fs[encode_itype_injective, encode_itype_o_f_injective]
-    )
+  rw[] >>
+  irule pure_unify_ind_lemma >>
+  simp[]
 QED
 
 Definition pure_apply_subst_def[nocompute]:
   pure_apply_subst s t =
-    THE $ decode_utype $ subst_APPLY (encode_itype o_f s) (encode_itype t)
+    decode_utype $ subst_APPLY (encode_itype o_f s) (encode_itype t)
 End
-
-Theorem pure_apply_subst_wf:
-  (∀t s. decode_utype $
-            subst_APPLY (encode_itype o_f s) (encode_itype t) ≠ NONE) ∧
-  (∀ts s. decode_utypes $
-            subst_APPLY (encode_itype o_f s) (encode_itypes ts) ≠ NONE)
-Proof
-  Induct >> rw[encode_itype_def, decode_utype_def, FLOOKUP_o_f] >>
-  CASE_TAC >> simp[decode_encode, decode_utype_def]
-QED
 
 Theorem pure_apply_subst:
   (∀s n.
-    pure_apply_subst s (CVar n) =
-      case FLOOKUP s n of | NONE => CVar n | SOME t => t) ∧
-  (∀s c ts.
-    pure_apply_subst s (TypeCons c ts) = TypeCons c (MAP (pure_apply_subst s) ts)) ∧
-  (∀s ts.
-    pure_apply_subst s (Tuple ts) = Tuple (MAP (pure_apply_subst s) ts)) ∧
-  (∀s t1 t2.
-    pure_apply_subst s (Function t1 t2) =
-      Function (pure_apply_subst s t1) (pure_apply_subst s t2)) ∧
+    pure_apply_subst s (iCVar n) =
+      case FLOOKUP s n of | NONE => iCVar n | SOME t => t) ∧
+  (∀s l r.
+    pure_apply_subst s (iCons l r) =
+    iCons (pure_apply_subst s l) (pure_apply_subst s r)) ∧
   (∀s t.
-    pure_apply_subst s (Array t) = Array (pure_apply_subst s t)) ∧
-  (∀s t.
-    pure_apply_subst s (M t) = M (pure_apply_subst s t)) ∧
-  (∀s n. pure_apply_subst s (DBVar n) = DBVar n) ∧
-  (∀s p. pure_apply_subst s (PrimTy p) = PrimTy p) ∧
-  (∀s. pure_apply_subst s Exception = Exception)
+    pure_apply_subst s (iAtom t) = iAtom t)
 Proof
   rw[pure_apply_subst_def, encode_itype_def, FLOOKUP_o_f, decode_utype_def] >>
-  every_case_tac >> rw[decode_encode, decode_utype_def]
-  >- (
-    Induct_on `ts` >> rw[encode_itype_def, decode_utype_def] >>
-    rw[pure_apply_subst_def, option_bind_case] >>
-    TOP_CASE_TAC >> gvs[pure_apply_subst_wf] >>
-    TOP_CASE_TAC >> gvs[pure_apply_subst_wf]
-    )
-  >- (
-    Induct_on `ts` >> rw[encode_itype_def, decode_utype_def] >>
-    rw[pure_apply_subst_def, option_bind_case] >>
-    TOP_CASE_TAC >> gvs[pure_apply_subst_wf] >>
-    TOP_CASE_TAC >> gvs[pure_apply_subst_wf]
-    )
-  >- (
-    rw[option_bind_case] >>
-    TOP_CASE_TAC >> gvs[pure_apply_subst_wf] >>
-    TOP_CASE_TAC >> gvs[pure_apply_subst_wf]
-    )
-  >- (
-    rw[option_bind_case] >>
-    qmatch_goalsub_abbrev_tac `decode_utype enc` >>
-    Cases_on `decode_utype enc` >> unabbrev_all_tac >> gvs[pure_apply_subst_wf]
-    )
-  >- (
-    rw[option_bind_case] >>
-    qmatch_goalsub_abbrev_tac `decode_utype enc` >>
-    Cases_on `decode_utype enc` >> unabbrev_all_tac >> gvs[pure_apply_subst_wf]
-    )
+  CASE_TAC >>
+  rw[decode_encode, decode_utype_def]
 QED
 
 Theorem walkstar_strongind:
@@ -1125,70 +434,47 @@ QED
 
 Definition pure_walkstar_def[nocompute]:
   pure_walkstar s t =
-    THE o decode_utype $ walkstar (encode_itype o_f s) (encode_itype t)
+    decode_utype $ walkstar (encode_itype o_f s) (encode_itype t)
 End
 
-Theorem pure_walkstar_ind:
+Triviality pure_walkstar_ind_lemma:
  ∀s. pure_wfs s ⇒
   ∀P.
     (∀t.
-      (∀c ts a. pure_walk s t = TypeCons c ts ∧ MEM a ts ⇒ P a) ∧
-      (∀ts a. pure_walk s t = Tuple ts ∧ MEM a ts ⇒ P a) ∧
-      (∀t1 t2. pure_walk s t = Function t1 t2 ⇒ P t1 ∧ P t2) ∧
-      (∀t'. pure_walk s t = Array t' ⇒ P t') ∧
-      (∀t'. pure_walk s t = M t' ⇒ P t')
+      (∀l r. pure_walk s t = iCons l r ⇒ P l ∧ P r)
+     ⇒ P t)
+  ⇒ ∀ut. ∀t. ut = encode_itype t ⇒ P t
+Proof
+  ntac 4 strip_tac >>
+  imp_res_tac pure_wfs_def >>
+  drule_then assume_tac $ GEN_ALL $ DISCH_ALL walkstar_ind >>
+  pop_assum $ qspec_then
+    `λut. ∀t. ut = encode_itype t ⇒ P t`
+    (assume_tac o SRULE[]) >>
+  rpt strip_tac >>
+  first_x_assum irule >>
+  fs[FORALL_AND_THM,IMP_CONJ_THM] >>
+  rw[] >>
+  last_x_assum irule >>
+  rw[]
+  >- (last_x_assum irule >>
+    simp[encode_walk,encode_itype_def]) >>
+  first_x_assum irule >>
+  simp[encode_walk,encode_itype_def]
+QED
+
+Theorem pure_walkstar_ind:
+  ∀s. pure_wfs s ⇒
+  ∀P.
+    (∀t.
+      (∀l r. pure_walk s t = iCons l r ⇒ P l ∧ P r)
      ⇒ P t)
   ⇒ ∀t. P t
 Proof
-  rw[] >> imp_res_tac pure_wfs_def >>
-  imp_res_tac $ GEN_ALL $ DISCH_ALL walkstar_ind >>
-  qsuff_tac `(λx.
-    (∀u. x = encode_itype u ⇒ P u) ∧
-    (∀c us. x = Pair (Const (uTypeCons c)) (encode_itypes us) ⇒ EVERY P us) ∧
-    (∀us. x = Pair (Const uTuple) (encode_itypes us) ⇒ EVERY P us) ∧
-    (∀u1 u2. x = Pair (Const uFunction)
-                  (Pair (encode_itype u1) (encode_itype u2)) ⇒ P u1 ∧ P u2) ∧
-    (∀u. x = Pair (Const uArray) (encode_itype u) ⇒ P u) ∧
-    (∀u. x = Pair (Const uM) (encode_itype u) ⇒ P u) ∧
-    (∀u1 u2. x = Pair (encode_itype u1) (encode_itype u2) ⇒ P u1 ∧ P u2) ∧
-    (∀u us. x = Pair (encode_itype u) (encode_itypes us) ⇒ EVERY P (u::us)))
-      (encode_itype t)`
-  >- simp[decode_encode] >>
-  pop_assum irule >> BETA_TAC >> rw[decode_encode]
-  >- (
-    rfs[encode_walk] >> first_x_assum irule >> rw[] >>
-    gvs[encode_walk, encode_itype_def, encode_itype_injective, EVERY_MEM] >>
-    Cases_on `ts` >> gvs[encode_itype_def, encode_itype_injective, EVERY_MEM]
-    )
-  >- (Cases_on `us` >> fs[encode_itype_def, encode_itype_injective])
-  >- (Cases_on `us` >> fs[encode_itype_def, encode_itype_injective]) >>
-  rfs[encode_walk, encode_itype_injective] >>
-  Cases_on `us` >> fs[encode_itype_def, encode_itype_injective]
-QED
-
-Theorem pure_walkstar_wf_lemma:
-  ∀s. pure_wfs s ⇒
-    ∀t. decode_utype $ walkstar (encode_itype o_f s) (encode_itype t) ≠ NONE
-Proof
-  strip_tac >> strip_tac >>
-  imp_res_tac pure_walkstar_ind >> pop_assum ho_match_mp_tac >> rw[] >>
-  imp_res_tac pure_wfs_def >> simp[Once walkstar_def, encode_walk] >>
-  Cases_on `pure_walk s t` >> gvs[encode_itype_def, decode_utype_def] >>
-  pop_assum kall_tac >> Induct_on `l` >> rw[encode_itype_def, decode_utype_def]
-QED
-
-Theorem pure_walkstar_wf:
-  (∀t s. pure_wfs s ⇒
-    decode_utype $
-      walkstar (encode_itype o_f s) (encode_itype t) ≠ NONE) ∧
-  (∀ts s. pure_wfs s ⇒
-    decode_utypes $
-      walkstar (encode_itype o_f s) (encode_itypes ts) ≠ NONE)
-Proof
-  conj_tac >- simp[pure_walkstar_wf_lemma] >>
-  Induct >> rw[] >> imp_res_tac pure_wfs_def >>
-  simp[encode_itype_def, decode_utype_def, Once walkstar_def] >>
-  irule pure_walkstar_wf_lemma >> simp[]
+  rw[] >>
+  irule pure_walkstar_ind_lemma >>
+  simp[] >>
+  metis_tac[]
 QED
 
 Theorem pure_walkstar_ts_lemma:
